refactor: make `extractLsb'` the primitive bv_decide understands, rather than `extractLsb`

src/Std/Tactic/BVDecide/Bitblast/BVExpr/Basic.lean
@@ -202,7 +202,7 @@ inductive BVExpr : Nat → Type where
   /--
   Extract a slice from a `BitVec`.
   -/
-  | extract (hi lo : Nat) (expr : BVExpr w) : BVExpr (hi - lo + 1)
+  | extract (start len : Nat) (expr : BVExpr w) : BVExpr len
   /--
   A binary operation on two `BVExpr`.
   -/
@@ -277,7 +277,7 @@ def eval (assign : Assignment) : BVExpr w → BitVec w
     bv.truncate w
   | .const val => val
   | .zeroExtend v expr => BitVec.zeroExtend v (eval assign expr)
-  | .extract hi lo expr => BitVec.extractLsb hi lo (eval assign expr)
+  | .extract start len expr => BitVec.extractLsb' start len (eval assign expr)
   | .bin lhs op rhs => op.eval (eval assign lhs) (eval assign rhs)
   | .un op operand => op.eval (eval assign operand)
   | .append lhs rhs => (eval assign lhs) ++ (eval assign rhs)
@@ -298,7 +298,7 @@ theorem eval_zeroExtend : eval assign (.zeroExtend v expr) = BitVec.zeroExtend v
   rfl
 
 @[simp]
-theorem eval_extract : eval assign (.extract hi lo expr) = BitVec.extractLsb hi lo (eval assign expr) := by
+theorem eval_extract : eval assign (.extract start len expr) = BitVec.extractLsb' start len (eval assign expr) := by
   rfl
 
 @[simp]
