src/Std/Tactic/BVDecide/Normalize/BitVec.lean
@@ -35,6 +35,7 @@ theorem BitVec.truncate_eq_zeroExtend (x : BitVec w) : x.truncate n = x.zeroExte
   rfl
 
 attribute [bv_normalize] BitVec.msb_eq_getLsb_last
+attribute [bv_normalize] BitVec.extractLsb
 attribute [bv_normalize] BitVec.slt_eq_ult
 attribute [bv_normalize] BitVec.sle_eq_not_slt
 
